UnreachableCode.v
@@ -6,45 +6,45 @@ Set Implicit Arguments.
 
 Local Hint Resolve incl_empty minus_incl incl_right incl_left.
 
-Inductive unreachable_code_precise
+Inductive unreachable_code
   : list params -> list bool -> stmt -> ann bool -> Prop :=
 | UCPOpr ZL Lv x b lv e al
-  :  unreachable_code_precise ZL Lv b al
-     -> unreachable_code_precise ZL Lv (stmtLet x e b) (ann1 lv al)
+  :  unreachable_code ZL Lv b al
+     -> unreachable_code ZL Lv (stmtLet x e b) (ann1 lv al)
 | UCPIf ZL Lv e b1 b2 lv al1 al2
-  :  (exp2bool e <> Some false -> unreachable_code_precise ZL Lv b1 al1)
-     -> (exp2bool e <> Some true -> unreachable_code_precise ZL Lv b2 al2)
-     -> unreachable_code_precise ZL Lv (stmtIf e b1 b2) (ann2 lv al1 al2)
+  :  (exp2bool e <> Some false -> unreachable_code ZL Lv b1 al1)
+     -> (exp2bool e <> Some true -> unreachable_code ZL Lv b2 al2)
+     -> unreachable_code ZL Lv (stmtIf e b1 b2) (ann2 lv al1 al2)
 | UCPGoto ZL Lv l Y lv Z
   : get ZL (counted l) Z
     -> get Lv (counted l) true
     -> length Y = length Z
-    -> unreachable_code_precise ZL Lv (stmtApp l Y) (ann0 lv)
+    -> unreachable_code ZL Lv (stmtApp l Y) (ann0 lv)
 | UCReturn ZL Lv e lv
-  : unreachable_code_precise ZL Lv (stmtReturn e) (ann0 lv)
+  : unreachable_code ZL Lv (stmtReturn e) (ann0 lv)
 | UCExtern ZL Lv x b lv Y al f
-  : unreachable_code_precise ZL Lv b al
-    -> unreachable_code_precise ZL Lv (stmtExtern x f Y b) (ann1 lv al)
+  : unreachable_code ZL Lv b al
+    -> unreachable_code ZL Lv (stmtExtern x f Y b) (ann1 lv al)
 | UCLet ZL Lv F t lv als alt
-  : unreachable_code_precise (fst ⊝ F ++ ZL) (getAnn ⊝ als ++ Lv) t alt
+  : unreachable_code (fst ⊝ F ++ ZL) (getAnn ⊝ als ++ Lv) t alt
     -> length F = length als
     -> (forall n Zs a, get F n Zs ->
                  get als n a ->
-                 unreachable_code_precise (fst ⊝ F ++ ZL) (getAnn ⊝ als ++ Lv) (snd Zs) a)
+                 unreachable_code (fst ⊝ F ++ ZL) (getAnn ⊝ als ++ Lv) (snd Zs) a)
     -> (forall n Zs a, get F n Zs ->
                  get als n a ->
                  getAnn a ->
                  trueIsCalled t (LabI n))
-    -> unreachable_code_precise ZL Lv (stmtFun F t) (annF lv als alt).
+    -> unreachable_code ZL Lv (stmtFun F t) (annF lv als alt).
 
 
-Lemma unreachable_code_precise_trueIsCalled i Lv s slv l
-  : unreachable_code_precise i Lv s slv
+Lemma unreachable_code_trueIsCalled i Lv s slv l
+  : unreachable_code i Lv s slv
     -> trueIsCalled s l
     -> get Lv (counted l) true.
 Proof.
   intros Live IC. destruct l; simpl in *.
-  general induction IC; invt unreachable_code_precise; eauto.
+  general induction IC; invt unreachable_code; eauto.
   - exploit IHIC2; eauto; simpl in *.
     rewrite get_app_lt in H1; eauto with len. inv_get.
     exploit IHIC1; eauto.
